Final Submission Candidate 1

.lake/build/ir/LeanIntro/Basic.c
@@ -1,0 +1,566 @@
+// Lean compiler output
+// Module: LeanIntro.Basic
+// Imports: Init
+#include <lean/lean.h>
+#if defined(__clang__)
+#pragma clang diagnostic ignored "-Wunused-parameter"
+#pragma clang diagnostic ignored "-Wunused-label"
+#elif defined(__GNUC__) && !defined(__CLANG__)
+#pragma GCC diagnostic ignored "-Wunused-parameter"
+#pragma GCC diagnostic ignored "-Wunused-label"
+#pragma GCC diagnostic ignored "-Wunused-but-set-variable"
+#endif
+#ifdef __cplusplus
+extern "C" {
+#endif
+LEAN_EXPORT lean_object* l_instReprPoint(lean_object*);
+static lean_object* l___private_LeanIntro_Basic_0__reprPoint____x40_LeanIntro_Basic___hyg_63____rarg___closed__9;
+static lean_object* l_origin___closed__2;
+static lean_object* l___private_LeanIntro_Basic_0__reprPoint____x40_LeanIntro_Basic___hyg_63____rarg___closed__11;
+static lean_object* l___private_LeanIntro_Basic_0__reprPoint____x40_LeanIntro_Basic___hyg_63____rarg___closed__5;
+static double l_distance___closed__1;
+LEAN_EXPORT lean_object* l_plusOneX(lean_object*);
+LEAN_EXPORT lean_object* l_instReprPoint___rarg(lean_object*);
+static lean_object* l___private_LeanIntro_Basic_0__reprPoint____x40_LeanIntro_Basic___hyg_63____rarg___closed__17;
+static lean_object* l___private_LeanIntro_Basic_0__reprPoint____x40_LeanIntro_Basic___hyg_63____rarg___closed__6;
+static lean_object* l___private_LeanIntro_Basic_0__reprPoint____x40_LeanIntro_Basic___hyg_63____rarg___closed__15;
+LEAN_EXPORT lean_object* l___private_LeanIntro_Basic_0__reprPoint____x40_LeanIntro_Basic___hyg_63____rarg___boxed(lean_object*, lean_object*, lean_object*);
+LEAN_EXPORT lean_object* l_origin___closed__2___boxed__const__1;
+LEAN_EXPORT lean_object* l___private_LeanIntro_Basic_0__reprPoint____x40_LeanIntro_Basic___hyg_63_(lean_object*);
+LEAN_EXPORT lean_object* l_sub1(lean_object*);
+double sqrt(double);
+LEAN_EXPORT lean_object* l_sub1___boxed(lean_object*);
+double lean_float_add(double, double);
+lean_object* lean_nat_to_int(lean_object*);
+LEAN_EXPORT lean_object* l_hello;
+static lean_object* l___private_LeanIntro_Basic_0__reprPoint____x40_LeanIntro_Basic___hyg_63____rarg___closed__8;
+static lean_object* l___private_LeanIntro_Basic_0__reprPoint____x40_LeanIntro_Basic___hyg_63____rarg___closed__1;
+static lean_object* l___private_LeanIntro_Basic_0__reprPoint____x40_LeanIntro_Basic___hyg_63____rarg___closed__2;
+static lean_object* l___private_LeanIntro_Basic_0__reprPoint____x40_LeanIntro_Basic___hyg_63____rarg___closed__13;
+double pow(double, double);
+LEAN_EXPORT lean_object* l_distance___boxed(lean_object*, lean_object*);
+static lean_object* l_hello___closed__1;
+lean_object* lean_int_sub(lean_object*, lean_object*);
+static lean_object* l___private_LeanIntro_Basic_0__reprPoint____x40_LeanIntro_Basic___hyg_63____rarg___closed__4;
+double l_Float_ofScientific(lean_object*, uint8_t, lean_object*);
+static lean_object* l___private_LeanIntro_Basic_0__reprPoint____x40_LeanIntro_Basic___hyg_63____rarg___closed__10;
+static lean_object* l___private_LeanIntro_Basic_0__reprPoint____x40_LeanIntro_Basic___hyg_63____rarg___closed__7;
+static lean_object* l___private_LeanIntro_Basic_0__reprPoint____x40_LeanIntro_Basic___hyg_63____rarg___closed__16;
+LEAN_EXPORT double l_distance(lean_object*, lean_object*);
+static double l_origin___closed__1;
+lean_object* lean_string_length(lean_object*);
+static lean_object* l___private_LeanIntro_Basic_0__reprPoint____x40_LeanIntro_Basic___hyg_63____rarg___closed__12;
+static lean_object* l_sub1___closed__1;
+LEAN_EXPORT lean_object* l___private_LeanIntro_Basic_0__reprPoint____x40_LeanIntro_Basic___hyg_63____rarg(lean_object*, lean_object*, lean_object*);
+static double l_plusOneX___closed__1;
+LEAN_EXPORT lean_object* l_origin;
+static lean_object* l___private_LeanIntro_Basic_0__reprPoint____x40_LeanIntro_Basic___hyg_63____rarg___closed__3;
+static lean_object* l___private_LeanIntro_Basic_0__reprPoint____x40_LeanIntro_Basic___hyg_63____rarg___closed__14;
+double lean_float_sub(double, double);
+static lean_object* _init_l_hello___closed__1() {
+_start:
+{
+lean_object* x_1; 
+x_1 = lean_mk_string_unchecked("world", 5, 5);
+return x_1;
+}
+}
+static lean_object* _init_l_hello() {
+_start:
+{
+lean_object* x_1; 
+x_1 = l_hello___closed__1;
+return x_1;
+}
+}
+static lean_object* _init_l_sub1___closed__1() {
+_start:
+{
+lean_object* x_1; lean_object* x_2; 
+x_1 = lean_unsigned_to_nat(1u);
+x_2 = lean_nat_to_int(x_1);
+return x_2;
+}
+}
+LEAN_EXPORT lean_object* l_sub1(lean_object* x_1) {
+_start:
+{
+lean_object* x_2; lean_object* x_3; 
+x_2 = l_sub1___closed__1;
+x_3 = lean_int_sub(x_1, x_2);
+return x_3;
+}
+}
+LEAN_EXPORT lean_object* l_sub1___boxed(lean_object* x_1) {
+_start:
+{
+lean_object* x_2; 
+x_2 = l_sub1(x_1);
+lean_dec(x_1);
+return x_2;
+}
+}
+static lean_object* _init_l___private_LeanIntro_Basic_0__reprPoint____x40_LeanIntro_Basic___hyg_63____rarg___closed__1() {
+_start:
+{
+lean_object* x_1; 
+x_1 = lean_mk_string_unchecked("x", 1, 1);
+return x_1;
+}
+}
+static lean_object* _init_l___private_LeanIntro_Basic_0__reprPoint____x40_LeanIntro_Basic___hyg_63____rarg___closed__2() {
+_start:
+{
+lean_object* x_1; lean_object* x_2; 
+x_1 = l___private_LeanIntro_Basic_0__reprPoint____x40_LeanIntro_Basic___hyg_63____rarg___closed__1;
+x_2 = lean_alloc_ctor(3, 1, 0);
+lean_ctor_set(x_2, 0, x_1);
+return x_2;
+}
+}
+static lean_object* _init_l___private_LeanIntro_Basic_0__reprPoint____x40_LeanIntro_Basic___hyg_63____rarg___closed__3() {
+_start:
+{
+lean_object* x_1; lean_object* x_2; lean_object* x_3; 
+x_1 = lean_box(0);
+x_2 = l___private_LeanIntro_Basic_0__reprPoint____x40_LeanIntro_Basic___hyg_63____rarg___closed__2;
+x_3 = lean_alloc_ctor(5, 2, 0);
+lean_ctor_set(x_3, 0, x_1);
+lean_ctor_set(x_3, 1, x_2);
+return x_3;
+}
+}
+static lean_object* _init_l___private_LeanIntro_Basic_0__reprPoint____x40_LeanIntro_Basic___hyg_63____rarg___closed__4() {
+_start:
+{
+lean_object* x_1; 
+x_1 = lean_mk_string_unchecked(" := ", 4, 4);
+return x_1;
+}
+}
+static lean_object* _init_l___private_LeanIntro_Basic_0__reprPoint____x40_LeanIntro_Basic___hyg_63____rarg___closed__5() {
+_start:
+{
+lean_object* x_1; lean_object* x_2; 
+x_1 = l___private_LeanIntro_Basic_0__reprPoint____x40_LeanIntro_Basic___hyg_63____rarg___closed__4;
+x_2 = lean_alloc_ctor(3, 1, 0);
+lean_ctor_set(x_2, 0, x_1);
+return x_2;
+}
+}
+static lean_object* _init_l___private_LeanIntro_Basic_0__reprPoint____x40_LeanIntro_Basic___hyg_63____rarg___closed__6() {
+_start:
+{
+lean_object* x_1; lean_object* x_2; lean_object* x_3; 
+x_1 = l___private_LeanIntro_Basic_0__reprPoint____x40_LeanIntro_Basic___hyg_63____rarg___closed__3;
+x_2 = l___private_LeanIntro_Basic_0__reprPoint____x40_LeanIntro_Basic___hyg_63____rarg___closed__5;
+x_3 = lean_alloc_ctor(5, 2, 0);
+lean_ctor_set(x_3, 0, x_1);
+lean_ctor_set(x_3, 1, x_2);
+return x_3;
+}
+}
+static lean_object* _init_l___private_LeanIntro_Basic_0__reprPoint____x40_LeanIntro_Basic___hyg_63____rarg___closed__7() {
+_start:
+{
+lean_object* x_1; lean_object* x_2; 
+x_1 = lean_unsigned_to_nat(5u);
+x_2 = lean_nat_to_int(x_1);
+return x_2;
+}
+}
+static lean_object* _init_l___private_LeanIntro_Basic_0__reprPoint____x40_LeanIntro_Basic___hyg_63____rarg___closed__8() {
+_start:
+{
+lean_object* x_1; 
+x_1 = lean_mk_string_unchecked(",", 1, 1);
+return x_1;
+}
+}
+static lean_object* _init_l___private_LeanIntro_Basic_0__reprPoint____x40_LeanIntro_Basic___hyg_63____rarg___closed__9() {
+_start:
+{
+lean_object* x_1; lean_object* x_2; 
+x_1 = l___private_LeanIntro_Basic_0__reprPoint____x40_LeanIntro_Basic___hyg_63____rarg___closed__8;
+x_2 = lean_alloc_ctor(3, 1, 0);
+lean_ctor_set(x_2, 0, x_1);
+return x_2;
+}
+}
+static lean_object* _init_l___private_LeanIntro_Basic_0__reprPoint____x40_LeanIntro_Basic___hyg_63____rarg___closed__10() {
+_start:
+{
+lean_object* x_1; 
+x_1 = lean_mk_string_unchecked("y", 1, 1);
+return x_1;
+}
+}
+static lean_object* _init_l___private_LeanIntro_Basic_0__reprPoint____x40_LeanIntro_Basic___hyg_63____rarg___closed__11() {
+_start:
+{
+lean_object* x_1; lean_object* x_2; 
+x_1 = l___private_LeanIntro_Basic_0__reprPoint____x40_LeanIntro_Basic___hyg_63____rarg___closed__10;
+x_2 = lean_alloc_ctor(3, 1, 0);
+lean_ctor_set(x_2, 0, x_1);
+return x_2;
+}
+}
+static lean_object* _init_l___private_LeanIntro_Basic_0__reprPoint____x40_LeanIntro_Basic___hyg_63____rarg___closed__12() {
+_start:
+{
+lean_object* x_1; 
+x_1 = lean_mk_string_unchecked("{ ", 2, 2);
+return x_1;
+}
+}
+static lean_object* _init_l___private_LeanIntro_Basic_0__reprPoint____x40_LeanIntro_Basic___hyg_63____rarg___closed__13() {
+_start:
+{
+lean_object* x_1; lean_object* x_2; 
+x_1 = l___private_LeanIntro_Basic_0__reprPoint____x40_LeanIntro_Basic___hyg_63____rarg___closed__12;
+x_2 = lean_string_length(x_1);
+return x_2;
+}
+}
+static lean_object* _init_l___private_LeanIntro_Basic_0__reprPoint____x40_LeanIntro_Basic___hyg_63____rarg___closed__14() {
+_start:
+{
+lean_object* x_1; lean_object* x_2; 
+x_1 = l___private_LeanIntro_Basic_0__reprPoint____x40_LeanIntro_Basic___hyg_63____rarg___closed__13;
+x_2 = lean_nat_to_int(x_1);
+return x_2;
+}
+}
+static lean_object* _init_l___private_LeanIntro_Basic_0__reprPoint____x40_LeanIntro_Basic___hyg_63____rarg___closed__15() {
+_start:
+{
+lean_object* x_1; lean_object* x_2; 
+x_1 = l___private_LeanIntro_Basic_0__reprPoint____x40_LeanIntro_Basic___hyg_63____rarg___closed__12;
+x_2 = lean_alloc_ctor(3, 1, 0);
+lean_ctor_set(x_2, 0, x_1);
+return x_2;
+}
+}
+static lean_object* _init_l___private_LeanIntro_Basic_0__reprPoint____x40_LeanIntro_Basic___hyg_63____rarg___closed__16() {
+_start:
+{
+lean_object* x_1; 
+x_1 = lean_mk_string_unchecked(" }", 2, 2);
+return x_1;
+}
+}
+static lean_object* _init_l___private_LeanIntro_Basic_0__reprPoint____x40_LeanIntro_Basic___hyg_63____rarg___closed__17() {
+_start:
+{
+lean_object* x_1; lean_object* x_2; 
+x_1 = l___private_LeanIntro_Basic_0__reprPoint____x40_LeanIntro_Basic___hyg_63____rarg___closed__16;
+x_2 = lean_alloc_ctor(3, 1, 0);
+lean_ctor_set(x_2, 0, x_1);
+return x_2;
+}
+}
+LEAN_EXPORT lean_object* l___private_LeanIntro_Basic_0__reprPoint____x40_LeanIntro_Basic___hyg_63____rarg(lean_object* x_1, lean_object* x_2, lean_object* x_3) {
+_start:
+{
+lean_object* x_4; lean_object* x_5; lean_object* x_6; lean_object* x_7; lean_object* x_8; uint8_t x_9; lean_object* x_10; lean_object* x_11; lean_object* x_12; lean_object* x_13; lean_object* x_14; lean_object* x_15; lean_object* x_16; lean_object* x_17; lean_object* x_18; lean_object* x_19; lean_object* x_20; lean_object* x_21; lean_object* x_22; lean_object* x_23; lean_object* x_24; lean_object* x_25; lean_object* x_26; lean_object* x_27; lean_object* x_28; lean_object* x_29; lean_object* x_30; lean_object* x_31; lean_object* x_32; 
+x_4 = lean_ctor_get(x_2, 0);
+lean_inc(x_4);
+x_5 = lean_unsigned_to_nat(0u);
+lean_inc(x_1);
+x_6 = lean_apply_2(x_1, x_4, x_5);
+x_7 = l___private_LeanIntro_Basic_0__reprPoint____x40_LeanIntro_Basic___hyg_63____rarg___closed__7;
+x_8 = lean_alloc_ctor(4, 2, 0);
+lean_ctor_set(x_8, 0, x_7);
+lean_ctor_set(x_8, 1, x_6);
+x_9 = 0;
+x_10 = lean_alloc_ctor(6, 1, 1);
+lean_ctor_set(x_10, 0, x_8);
+lean_ctor_set_uint8(x_10, sizeof(void*)*1, x_9);
+x_11 = l___private_LeanIntro_Basic_0__reprPoint____x40_LeanIntro_Basic___hyg_63____rarg___closed__6;
+x_12 = lean_alloc_ctor(5, 2, 0);
+lean_ctor_set(x_12, 0, x_11);
+lean_ctor_set(x_12, 1, x_10);
+x_13 = l___private_LeanIntro_Basic_0__reprPoint____x40_LeanIntro_Basic___hyg_63____rarg___closed__9;
+x_14 = lean_alloc_ctor(5, 2, 0);
+lean_ctor_set(x_14, 0, x_12);
+lean_ctor_set(x_14, 1, x_13);
+x_15 = lean_box(1);
+x_16 = lean_alloc_ctor(5, 2, 0);
+lean_ctor_set(x_16, 0, x_14);
+lean_ctor_set(x_16, 1, x_15);
+x_17 = l___private_LeanIntro_Basic_0__reprPoint____x40_LeanIntro_Basic___hyg_63____rarg___closed__11;
+x_18 = lean_alloc_ctor(5, 2, 0);
+lean_ctor_set(x_18, 0, x_16);
+lean_ctor_set(x_18, 1, x_17);
+x_19 = l___private_LeanIntro_Basic_0__reprPoint____x40_LeanIntro_Basic___hyg_63____rarg___closed__5;
+x_20 = lean_alloc_ctor(5, 2, 0);
+lean_ctor_set(x_20, 0, x_18);
+lean_ctor_set(x_20, 1, x_19);
+x_21 = lean_ctor_get(x_2, 1);
+lean_inc(x_21);
+lean_dec(x_2);
+x_22 = lean_apply_2(x_1, x_21, x_5);
+x_23 = lean_alloc_ctor(4, 2, 0);
+lean_ctor_set(x_23, 0, x_7);
+lean_ctor_set(x_23, 1, x_22);
+x_24 = lean_alloc_ctor(6, 1, 1);
+lean_ctor_set(x_24, 0, x_23);
+lean_ctor_set_uint8(x_24, sizeof(void*)*1, x_9);
+x_25 = lean_alloc_ctor(5, 2, 0);
+lean_ctor_set(x_25, 0, x_20);
+lean_ctor_set(x_25, 1, x_24);
+x_26 = l___private_LeanIntro_Basic_0__reprPoint____x40_LeanIntro_Basic___hyg_63____rarg___closed__15;
+x_27 = lean_alloc_ctor(5, 2, 0);
+lean_ctor_set(x_27, 0, x_26);
+lean_ctor_set(x_27, 1, x_25);
+x_28 = l___private_LeanIntro_Basic_0__reprPoint____x40_LeanIntro_Basic___hyg_63____rarg___closed__17;
+x_29 = lean_alloc_ctor(5, 2, 0);
+lean_ctor_set(x_29, 0, x_27);
+lean_ctor_set(x_29, 1, x_28);
+x_30 = l___private_LeanIntro_Basic_0__reprPoint____x40_LeanIntro_Basic___hyg_63____rarg___closed__14;
+x_31 = lean_alloc_ctor(4, 2, 0);
+lean_ctor_set(x_31, 0, x_30);
+lean_ctor_set(x_31, 1, x_29);
+x_32 = lean_alloc_ctor(6, 1, 1);
+lean_ctor_set(x_32, 0, x_31);
+lean_ctor_set_uint8(x_32, sizeof(void*)*1, x_9);
+return x_32;
+}
+}
+LEAN_EXPORT lean_object* l___private_LeanIntro_Basic_0__reprPoint____x40_LeanIntro_Basic___hyg_63_(lean_object* x_1) {
+_start:
+{
+lean_object* x_2; 
+x_2 = lean_alloc_closure((void*)(l___private_LeanIntro_Basic_0__reprPoint____x40_LeanIntro_Basic___hyg_63____rarg___boxed), 3, 0);
+return x_2;
+}
+}
+LEAN_EXPORT lean_object* l___private_LeanIntro_Basic_0__reprPoint____x40_LeanIntro_Basic___hyg_63____rarg___boxed(lean_object* x_1, lean_object* x_2, lean_object* x_3) {
+_start:
+{
+lean_object* x_4; 
+x_4 = l___private_LeanIntro_Basic_0__reprPoint____x40_LeanIntro_Basic___hyg_63____rarg(x_1, x_2, x_3);
+lean_dec(x_3);
+return x_4;
+}
+}
+LEAN_EXPORT lean_object* l_instReprPoint___rarg(lean_object* x_1) {
+_start:
+{
+lean_object* x_2; 
+x_2 = lean_alloc_closure((void*)(l___private_LeanIntro_Basic_0__reprPoint____x40_LeanIntro_Basic___hyg_63____rarg___boxed), 3, 1);
+lean_closure_set(x_2, 0, x_1);
+return x_2;
+}
+}
+LEAN_EXPORT lean_object* l_instReprPoint(lean_object* x_1) {
+_start:
+{
+lean_object* x_2; 
+x_2 = lean_alloc_closure((void*)(l_instReprPoint___rarg), 1, 0);
+return x_2;
+}
+}
+static double _init_l_origin___closed__1() {
+_start:
+{
+lean_object* x_1; uint8_t x_2; lean_object* x_3; double x_4; 
+x_1 = lean_unsigned_to_nat(0u);
+x_2 = 1;
+x_3 = lean_unsigned_to_nat(1u);
+x_4 = l_Float_ofScientific(x_1, x_2, x_3);
+return x_4;
+}
+}
+static lean_object* _init_l_origin___closed__2___boxed__const__1() {
+_start:
+{
+double x_1; lean_object* x_2; 
+x_1 = l_origin___closed__1;
+x_2 = lean_box_float(x_1);
+return x_2;
+}
+}
+static lean_object* _init_l_origin___closed__2() {
+_start:
+{
+lean_object* x_1; lean_object* x_2; lean_object* x_3; 
+x_1 = l_origin___closed__2___boxed__const__1;
+x_2 = l_origin___closed__2___boxed__const__1;
+x_3 = lean_alloc_ctor(0, 2, 0);
+lean_ctor_set(x_3, 0, x_1);
+lean_ctor_set(x_3, 1, x_2);
+return x_3;
+}
+}
+static lean_object* _init_l_origin() {
+_start:
+{
+lean_object* x_1; 
+x_1 = l_origin___closed__2;
+return x_1;
+}
+}
+static double _init_l_distance___closed__1() {
+_start:
+{
+lean_object* x_1; uint8_t x_2; lean_object* x_3; double x_4; 
+x_1 = lean_unsigned_to_nat(20u);
+x_2 = 1;
+x_3 = lean_unsigned_to_nat(1u);
+x_4 = l_Float_ofScientific(x_1, x_2, x_3);
+return x_4;
+}
+}
+LEAN_EXPORT double l_distance(lean_object* x_1, lean_object* x_2) {
+_start:
+{
+lean_object* x_3; lean_object* x_4; double x_5; double x_6; double x_7; double x_8; double x_9; lean_object* x_10; lean_object* x_11; double x_12; double x_13; double x_14; double x_15; double x_16; double x_17; 
+x_3 = lean_ctor_get(x_2, 0);
+lean_inc(x_3);
+x_4 = lean_ctor_get(x_1, 0);
+lean_inc(x_4);
+x_5 = lean_unbox_float(x_3);
+lean_dec(x_3);
+x_6 = lean_unbox_float(x_4);
+lean_dec(x_4);
+x_7 = lean_float_sub(x_5, x_6);
+x_8 = l_distance___closed__1;
+x_9 = pow(x_7, x_8);
+x_10 = lean_ctor_get(x_2, 1);
+lean_inc(x_10);
+lean_dec(x_2);
+x_11 = lean_ctor_get(x_1, 1);
+lean_inc(x_11);
+lean_dec(x_1);
+x_12 = lean_unbox_float(x_10);
+lean_dec(x_10);
+x_13 = lean_unbox_float(x_11);
+lean_dec(x_11);
+x_14 = lean_float_sub(x_12, x_13);
+x_15 = pow(x_14, x_8);
+x_16 = lean_float_add(x_9, x_15);
+x_17 = sqrt(x_16);
+return x_17;
+}
+}
+LEAN_EXPORT lean_object* l_distance___boxed(lean_object* x_1, lean_object* x_2) {
+_start:
+{
+double x_3; lean_object* x_4; 
+x_3 = l_distance(x_1, x_2);
+x_4 = lean_box_float(x_3);
+return x_4;
+}
+}
+static double _init_l_plusOneX___closed__1() {
+_start:
+{
+lean_object* x_1; uint8_t x_2; lean_object* x_3; double x_4; 
+x_1 = lean_unsigned_to_nat(10u);
+x_2 = 1;
+x_3 = lean_unsigned_to_nat(1u);
+x_4 = l_Float_ofScientific(x_1, x_2, x_3);
+return x_4;
+}
+}
+LEAN_EXPORT lean_object* l_plusOneX(lean_object* x_1) {
+_start:
+{
+uint8_t x_2; 
+x_2 = !lean_is_exclusive(x_1);
+if (x_2 == 0)
+{
+lean_object* x_3; double x_4; double x_5; double x_6; lean_object* x_7; 
+x_3 = lean_ctor_get(x_1, 0);
+x_4 = l_plusOneX___closed__1;
+x_5 = lean_unbox_float(x_3);
+lean_dec(x_3);
+x_6 = lean_float_add(x_5, x_4);
+x_7 = lean_box_float(x_6);
+lean_ctor_set(x_1, 0, x_7);
+return x_1;
+}
+else
+{
+lean_object* x_8; lean_object* x_9; double x_10; double x_11; double x_12; lean_object* x_13; lean_object* x_14; 
+x_8 = lean_ctor_get(x_1, 0);
+x_9 = lean_ctor_get(x_1, 1);
+lean_inc(x_9);
+lean_inc(x_8);
+lean_dec(x_1);
+x_10 = l_plusOneX___closed__1;
+x_11 = lean_unbox_float(x_8);
+lean_dec(x_8);
+x_12 = lean_float_add(x_11, x_10);
+x_13 = lean_box_float(x_12);
+x_14 = lean_alloc_ctor(0, 2, 0);
+lean_ctor_set(x_14, 0, x_13);
+lean_ctor_set(x_14, 1, x_9);
+return x_14;
+}
+}
+}
+lean_object* initialize_Init(uint8_t builtin, lean_object*);
+static bool _G_initialized = false;
+LEAN_EXPORT lean_object* initialize_LeanIntro_Basic(uint8_t builtin, lean_object* w) {
+lean_object * res;
+if (_G_initialized) return lean_io_result_mk_ok(lean_box(0));
+_G_initialized = true;
+res = initialize_Init(builtin, lean_io_mk_world());
+if (lean_io_result_is_error(res)) return res;
+lean_dec_ref(res);
+l_hello___closed__1 = _init_l_hello___closed__1();
+lean_mark_persistent(l_hello___closed__1);
+l_hello = _init_l_hello();
+lean_mark_persistent(l_hello);
+l_sub1___closed__1 = _init_l_sub1___closed__1();
+lean_mark_persistent(l_sub1___closed__1);
+l___private_LeanIntro_Basic_0__reprPoint____x40_LeanIntro_Basic___hyg_63____rarg___closed__1 = _init_l___private_LeanIntro_Basic_0__reprPoint____x40_LeanIntro_Basic___hyg_63____rarg___closed__1();
+lean_mark_persistent(l___private_LeanIntro_Basic_0__reprPoint____x40_LeanIntro_Basic___hyg_63____rarg___closed__1);
+l___private_LeanIntro_Basic_0__reprPoint____x40_LeanIntro_Basic___hyg_63____rarg___closed__2 = _init_l___private_LeanIntro_Basic_0__reprPoint____x40_LeanIntro_Basic___hyg_63____rarg___closed__2();
+lean_mark_persistent(l___private_LeanIntro_Basic_0__reprPoint____x40_LeanIntro_Basic___hyg_63____rarg___closed__2);
+l___private_LeanIntro_Basic_0__reprPoint____x40_LeanIntro_Basic___hyg_63____rarg___closed__3 = _init_l___private_LeanIntro_Basic_0__reprPoint____x40_LeanIntro_Basic___hyg_63____rarg___closed__3();
+lean_mark_persistent(l___private_LeanIntro_Basic_0__reprPoint____x40_LeanIntro_Basic___hyg_63____rarg___closed__3);
+l___private_LeanIntro_Basic_0__reprPoint____x40_LeanIntro_Basic___hyg_63____rarg___closed__4 = _init_l___private_LeanIntro_Basic_0__reprPoint____x40_LeanIntro_Basic___hyg_63____rarg___closed__4();
+lean_mark_persistent(l___private_LeanIntro_Basic_0__reprPoint____x40_LeanIntro_Basic___hyg_63____rarg___closed__4);
+l___private_LeanIntro_Basic_0__reprPoint____x40_LeanIntro_Basic___hyg_63____rarg___closed__5 = _init_l___private_LeanIntro_Basic_0__reprPoint____x40_LeanIntro_Basic___hyg_63____rarg___closed__5();
+lean_mark_persistent(l___private_LeanIntro_Basic_0__reprPoint____x40_LeanIntro_Basic___hyg_63____rarg___closed__5);
+l___private_LeanIntro_Basic_0__reprPoint____x40_LeanIntro_Basic___hyg_63____rarg___closed__6 = _init_l___private_LeanIntro_Basic_0__reprPoint____x40_LeanIntro_Basic___hyg_63____rarg___closed__6();
+lean_mark_persistent(l___private_LeanIntro_Basic_0__reprPoint____x40_LeanIntro_Basic___hyg_63____rarg___closed__6);
+l___private_LeanIntro_Basic_0__reprPoint____x40_LeanIntro_Basic___hyg_63____rarg___closed__7 = _init_l___private_LeanIntro_Basic_0__reprPoint____x40_LeanIntro_Basic___hyg_63____rarg___closed__7();
+lean_mark_persistent(l___private_LeanIntro_Basic_0__reprPoint____x40_LeanIntro_Basic___hyg_63____rarg___closed__7);
+l___private_LeanIntro_Basic_0__reprPoint____x40_LeanIntro_Basic___hyg_63____rarg___closed__8 = _init_l___private_LeanIntro_Basic_0__reprPoint____x40_LeanIntro_Basic___hyg_63____rarg___closed__8();
+lean_mark_persistent(l___private_LeanIntro_Basic_0__reprPoint____x40_LeanIntro_Basic___hyg_63____rarg___closed__8);
+l___private_LeanIntro_Basic_0__reprPoint____x40_LeanIntro_Basic___hyg_63____rarg___closed__9 = _init_l___private_LeanIntro_Basic_0__reprPoint____x40_LeanIntro_Basic___hyg_63____rarg___closed__9();
+lean_mark_persistent(l___private_LeanIntro_Basic_0__reprPoint____x40_LeanIntro_Basic___hyg_63____rarg___closed__9);
+l___private_LeanIntro_Basic_0__reprPoint____x40_LeanIntro_Basic___hyg_63____rarg___closed__10 = _init_l___private_LeanIntro_Basic_0__reprPoint____x40_LeanIntro_Basic___hyg_63____rarg___closed__10();
+lean_mark_persistent(l___private_LeanIntro_Basic_0__reprPoint____x40_LeanIntro_Basic___hyg_63____rarg___closed__10);
+l___private_LeanIntro_Basic_0__reprPoint____x40_LeanIntro_Basic___hyg_63____rarg___closed__11 = _init_l___private_LeanIntro_Basic_0__reprPoint____x40_LeanIntro_Basic___hyg_63____rarg___closed__11();
+lean_mark_persistent(l___private_LeanIntro_Basic_0__reprPoint____x40_LeanIntro_Basic___hyg_63____rarg___closed__11);
+l___private_LeanIntro_Basic_0__reprPoint____x40_LeanIntro_Basic___hyg_63____rarg___closed__12 = _init_l___private_LeanIntro_Basic_0__reprPoint____x40_LeanIntro_Basic___hyg_63____rarg___closed__12();
+lean_mark_persistent(l___private_LeanIntro_Basic_0__reprPoint____x40_LeanIntro_Basic___hyg_63____rarg___closed__12);
+l___private_LeanIntro_Basic_0__reprPoint____x40_LeanIntro_Basic___hyg_63____rarg___closed__13 = _init_l___private_LeanIntro_Basic_0__reprPoint____x40_LeanIntro_Basic___hyg_63____rarg___closed__13();
+lean_mark_persistent(l___private_LeanIntro_Basic_0__reprPoint____x40_LeanIntro_Basic___hyg_63____rarg___closed__13);
+l___private_LeanIntro_Basic_0__reprPoint____x40_LeanIntro_Basic___hyg_63____rarg___closed__14 = _init_l___private_LeanIntro_Basic_0__reprPoint____x40_LeanIntro_Basic___hyg_63____rarg___closed__14();
+lean_mark_persistent(l___private_LeanIntro_Basic_0__reprPoint____x40_LeanIntro_Basic___hyg_63____rarg___closed__14);
+l___private_LeanIntro_Basic_0__reprPoint____x40_LeanIntro_Basic___hyg_63____rarg___closed__15 = _init_l___private_LeanIntro_Basic_0__reprPoint____x40_LeanIntro_Basic___hyg_63____rarg___closed__15();
+lean_mark_persistent(l___private_LeanIntro_Basic_0__reprPoint____x40_LeanIntro_Basic___hyg_63____rarg___closed__15);
+l___private_LeanIntro_Basic_0__reprPoint____x40_LeanIntro_Basic___hyg_63____rarg___closed__16 = _init_l___private_LeanIntro_Basic_0__reprPoint____x40_LeanIntro_Basic___hyg_63____rarg___closed__16();
+lean_mark_persistent(l___private_LeanIntro_Basic_0__reprPoint____x40_LeanIntro_Basic___hyg_63____rarg___closed__16);
+l___private_LeanIntro_Basic_0__reprPoint____x40_LeanIntro_Basic___hyg_63____rarg___closed__17 = _init_l___private_LeanIntro_Basic_0__reprPoint____x40_LeanIntro_Basic___hyg_63____rarg___closed__17();
+lean_mark_persistent(l___private_LeanIntro_Basic_0__reprPoint____x40_LeanIntro_Basic___hyg_63____rarg___closed__17);
+l_origin___closed__1 = _init_l_origin___closed__1();
+l_origin___closed__2___boxed__const__1 = _init_l_origin___closed__2___boxed__const__1();
+lean_mark_persistent(l_origin___closed__2___boxed__const__1);
+l_origin___closed__2 = _init_l_origin___closed__2();
+lean_mark_persistent(l_origin___closed__2);
+l_origin = _init_l_origin();
+lean_mark_persistent(l_origin);
+l_distance___closed__1 = _init_l_distance___closed__1();
+l_plusOneX___closed__1 = _init_l_plusOneX___closed__1();
+return lean_io_result_mk_ok(lean_box(0));
+}
+#ifdef __cplusplus
+}
+#endif
