HISTORY.md
@@ -1,3 +1,24 @@
 # Project_2_431
 
 An introduction to the history of the Lean Programming Language
+
+Lean initially launched in 2013, developed by Leonardo de Moura while working at Microsoft Research. Versions 1 and 2 were largely experimental, and contained support for some features that were dropped in later versions of the language, including Homotopy Type Theory
+
+The first modern version of the language, Lean 3, launched in January of 2017 and was primarily implemented in C++. It continued to recieve official updates up to version 3.4.2, when official support ended to begin focus on developing Lean 4. However, community members did continue to push their own unofficial updates up to 3.51.1 during this development period.
+
+2021 saw the release of Lean 4, the most recent version of the language. Lean 4 is fully implemented in itself, meaning users on't need to interface with C++ code to change core functions of the language. Unlike some other languages, Lean is not backwards compatible with previous versions, meaning programs written in Lean 3 will not work in Lean 4.
+
+In 2023, the Lean Focused Research Organization was formed, a non-profit organization dedicated to the development of Lean. Their primary aims are increasing the scalability and usability of Lean, as well as implementing Proof Automation to further increase usefulness.
+
+The latest version of Lean is 4.14.0, released December 9th 2024.
+
+As of writing, noteworthy features of Lean include:
+ - Type Inference
+ - First-class functions
+ - Powerful types, Dependent types
+ - Type classes
+ - Pattern matching
+ - Macro system
+ - Metaprogramming framework
+ - Multithreading
+ - Single-Language Property Proving
