README.md
@@ -5,9 +5,15 @@ Each piece of the project will have its own .md file
 Example Code is within the LeanIntro folder within the Overall Project 2 Folder(Project_2_431/LeanIntro)
 This file will serve as a table of contents for these files
 
-File:               Contents:
-README.md           Current location. Project Directory
-INSTALL.md          WSL Installation guide and requirements
-HISTORY.md          Development History of Lean
-USAGE.md            Common Use Cases of Lean
-kanpilot.toml       Kanban Board config file. Ignore.
+File:                   Contents:
+README.md               Current location. Project Directory
+INSTALL.md              WSL Installation guide and requirements
+HISTORY.md              Development History and Future Plans for Lean
+USAGE.md                Design, Motivation, Use Cases, and Shortcomings of Lean
+LeanIntro/Basic.lean    Simple Lean Demo Program (with comments)
+kanpilot.toml           Kanban Board config file. Ignore.
+lakefile.lean      \
+lean-toolchain      |
+LeanIntro.lean      |---Lean project files. Ignore.
+lake-manifest.json  |
+.lake/             /
